WIP

cava/arrow-examples/Aes/cipher_properties.v
@@ -15,92 +15,174 @@ Local Notation INV_AES data key :=
   (combinational_evaluation'
      unrolled_cipher_naive (true, (data, (key, tt)))) (only parsing).
 
-(*
-Lemma combinational_evaluation'_proper
-      {CircuitLaws : CategoryLaws CircuitCat}
-      i o (c c' : Circuit i o) args :
-  c =M= c' ->
-  combinational_evaluation' c args = combinational_evaluation' c' args.
-Proof.
-Qed.
- *)
 Require Import Coq.Classes.Morphisms.
 
-Context {CircuitLaws : CategoryLaws CircuitCat}
-        {CircuitArrowLaws :
-           ArrowLaws Kind CircuitCat CircuitLaws Unit Tuple CircuitArrow}.
-
-About combinational_evaluation'.
-About morphism_equivalence.
-Locate "==>".
-About respectful.
-Print Relation_Definitions.relation.
-Print respectful.
-Definition test :
-  Relation_Definitions.relation
-    (forall i o : Kind, Circuit i o -> denote_kind i -> denote_kind o).
-Proof.
-  do 2 (eapply forall_relation; intros).
-  repeat eapply @respectful.
-  { exact (morphism_equivalence a a0). }
-  { exact Logic.eq. }
-  { exact Logic.eq. }
-Defined.
-Global Instance combinational_evaluation'_Proper :
+Global Instance combinational_evaluation'_Proper
+       {circuit_laws : CategoryLaws CircuitCat} :
   Proper  
     (forall_relation
        (fun i : Kind =>
           forall_relation
             (fun o : Kind =>
-               (morphism_equivalence i o) ==> Logic.eq ==> Logic.eq)))%signature
+               (morphism_equivalence i o)
+                 ==> Logic.eq ==> Logic.eq)))%signature
          (@combinational_evaluation').
 Admitted.
 
-Global Instance combinational_evaluation'_naive_cipher_unrolled_Proper :
+Global Instance combinational_evaluation'_naive_cipher_unrolled_Proper
+       {circuit_laws : CategoryLaws CircuitCat} :
   Proper (morphism_equivalence
             (Bit ** Vector Bit 128 ** Vector Bit 256 ** Unit)
             (Vector Bit 128) ==> Logic.eq ==> Logic.eq)
          combinational_evaluation'.
-Proof.
-  apply combinational_evaluation'_Proper.
-Qed.
+Proof. apply combinational_evaluation'_Proper. Qed.
 
-Global Instance combinational_evaluation'_swap_Proper :
-  Proper (morphism_equivalence
-            (Bit ** Bit)
-            (((Bit ** Bit) ** Unit) ** (Bit ** Bit) ** Unit)
-            ==> Logic.eq ==> Logic.eq)
-         combinational_evaluation'.
-Proof.
-  apply combinational_evaluation'_Proper.
-Qed.
-
-About compose.
 Global Instance compose_Proper
-       {object} {category : Category object} x y z :
+       {object} {category : Category object}
+       {category_laws : CategoryLaws category}
+       x y z :
   Proper ((morphism_equivalence y z) ==> (morphism_equivalence x y)
             ==> (morphism_equivalence x z))
          compose.
 Admitted.
 
-Check combinational_evaluation'_naive_cipher_unrolled_Proper.
-(* bit-swap has fast rewrite *)
-Goal (forall inp out k,
-         @combinational_evaluation'
-           (Bit ** Vector Bit (4 * 4 * 8) ** Vector Bit (8 * 4 * 8) ** Unit)
-           (Vector Bit (4 * 4 * 8))
-           (uncancelr >>> first swap >>> k)
-           (inp) = out).
+(* TODO: add something to categorylaws *)
+Global Instance first_Proper
+       {object category unit product}
+       {arrow : Arrow object category unit product}
+       {arrow_laws : CategoryLaws arrow}
+       {x y z : object} :
+  Proper ((morphism_equivalence x y)
+            ==> (morphism_equivalence (x ** z) (y ** z)))
+         first.
+Admitted.
+
+(* TODO: add something to categorylaws *)
+Global Instance second_Proper
+       {object category unit product}
+       {arrow : Arrow object category unit product}
+       {arrow_laws : CategoryLaws arrow}
+       {x y z : object} :
+  Proper ((morphism_equivalence x y)
+            ==> (morphism_equivalence (z ** x) (z ** y)))
+         second.
+Admitted.
+
+Context {CircuitLaws : CategoryLaws CircuitCat}
+        {CircuitArrowLaws :
+           ArrowLaws Kind CircuitCat CircuitLaws Unit Tuple CircuitArrow}.
+
+Goal (forall (f : Unit ~[CircuitCat]~> Unit)
+             (k : Unit ** Unit ~[_]~> Unit ** Unit)
+             m,
+         morphism_equivalence
+           <<Unit ** Unit>> <<(Unit ** Unit) ** Unit>>
+           (first (uncancell >>> second f >>> k))
+           (first m)).
 Proof.
   intros.
-  rewrite (uncancelr_first_cont (category:=CircuitCat)).
+  rewrite uncancell_second_cont.
 Abort.
 
-Lemma cipher_id data ekey dkey :
-  INV_AES (AES data ekey) dkey = data.
+Lemma first_first_cont
+       {object category unit product}
+       {arrow : Arrow object category unit product}
+       {arrow_laws : CategoryLaws arrow}
+       {v w x y z} (f : x ~> y) (g : y ~> z) (k : z ** w ~> v):
+  first f >>> first g >>> k =M= first (f >>> g) >>> k.
+Admitted.
+
+Lemma swap_swap
+       {object category unit product}
+       {arrow : Arrow object category unit product}
+       {arrow_laws : CategoryLaws arrow}
+       {x y}:
+  swap >>> swap =M= (id (x:=x **y)).
+Admitted.
+
+Lemma first_id_cont
+       {object category unit product}
+       {arrow : Arrow object category unit product}
+       {arrow_laws : CategoryLaws arrow}
+       {x y z} (k : x ** y ~> z):
+  first id >>> k =M= k.
+Admitted.
+
+Lemma unassoc_assoc_cont
+       {object category unit product}
+       {arrow : Arrow object category unit product}
+       {arrow_laws : CategoryLaws arrow}
+       {w x y z} (k : x ** y ** z ~> w) :
+  unassoc >>> assoc >>> k =M= k.
+Admitted.
+
+Lemma second_second_cont
+       {object category unit product}
+       {arrow : Arrow object category unit product}
+       {arrow_laws : CategoryLaws arrow}
+       {v w x y z} (f : x ~> y) (g : y ~> z) (k : w ** z ~> v):
+  second f >>> second g >>> k =M= second (f >>> g) >>> k.
+Admitted.
+
+Print fold_right.
+Eval cbn [List.fold_right List.seq] in (List.fold_right Nat.add 0 (List.seq 0 4)).
+Eval cbn [List.fold_left List.seq] in (List.fold_left Nat.add (List.seq 0 4) 0).
+Axiom xor_spec : list bool -> list bool -> list bool.
+Axiom sub_bytes_spec : list bool -> list bool.
+Axiom shift_rows_spec : list bool -> list bool.
+Axiom mix_columns_spec : list bool -> list bool.
+Axiom key_expand_spec : list bool -> list bool.
+Definition cipher_round_spec (data key : list bool) : list bool :=
+  let data := xor_spec data key in
+  let data := sub_bytes_spec data in
+  let data := shift_rows_spec data in
+  let data := mix_columns_spec data in
+  data.
+Definition aes_cipher_spec
+           (nrounds : nat)
+           (data key : list bool) : list bool :=
+  (* first xor *)
+  let data := xor_spec data key in
+  let key := key_expand_spec key in
+  (* main loop *)
+  let st :=
+      List.fold_left (fun st _ =>
+                        let data := fst st in
+                        let key := snd st in
+                        (cipher_round_spec data key, key_expand_spec key))
+                     (List.seq 0 nrounds) (data, key) in
+  let data := fst st in
+  let key := snd st in
+  (* final cipher round *)
+  let data := xor_spec data key in
+  let data := sub_bytes_spec data in
+  let data := shift_rows_spec data in
+  data.
+
+About unrolled_cipher_naive.
+Search t list.
+Lemma unrolled_cipher_naive_equiv n data key :
+  to_list (AES data key) = aes_cipher_spec n (to_list data) (to_list key).
 Proof.
   cbn [denote_kind] in *.
-  unfold unrolled_cipher_naive at 1.
+  unfold unrolled_cipher_naive.
+  change 256 with (4 * 8 * 8).
+  change 128 with (4 * 4 * 8).
+  rewrite expression_evaluation_is_arrow_evaluation.
+  cbn [interp_combinational].
+  Print reshape.
+  (* What is needed to prove the id lemma with kappa/arrows?
+     What is needed to prove the id lemma with monads?
+     What about the equivalence?
+     experiment with all 4?
+ *)
+     
+  Set Printing Implicit.
+
+Lemma cipher_id data ekey dkey : INV_AES (AES data ekey) dkey = data.
+Proof.
+  cbn [denote_kind] in *.
+  unfold unrolled_cipher_naive at 1 2.
   change 256 with (4 * 8 * 8).
   change 128 with (4 * 4 * 8).
   cbv [ClosureConversion.closure_conversion].
@@ -121,6 +203,53 @@ Proof.
   erewrite combinational_evaluation'_Proper.
   3:reflexivity.
   2:{
+    Hint Rewrite
+         @first_cancelr_cont
+         @second_cancell_cont
+         @uncancelr_first_cont
+         @uncancell_second_cont using solve [typeclasses eauto]
+    : arrowlaws.
     Time
-      rewrite (uncancelr_first_cont (category:=CircuitCat)).
-    Search copy.
+      autorewrite with arrowlaws.
+    repeat match goal with
+           | |- context [first (?a >>> ?b)] =>
+             let f := fresh "f" in
+             set (f:=(a >>> b))
+           | |- context [second (?a >>> ?b)] =>
+             let f := fresh "f" in
+             set (f:=(a >>> b))
+           end.
+    rewrite first_first_cont.
+    rewrite swap_swap.
+    rewrite first_id_cont.
+    rewrite unassoc_assoc_cont.
+    rewrite second_second_cont.
+    (*
+      input :
+      << Bit ** (Vector Bit (4 * 4 * 8)
+         ** (Vector Bit (4 * 8 * 8) ** Unit >>
+                    (op_i, (data, (key, tt)))
+  swap >>>          ((data, (key, tt)), op_i)
+  uncancelr >>>     (((data, (key, tt)), op_i), tt)
+  assoc >>>         ((data, (key, tt)), (op_i, tt))
+  first swap >>>    (((key, tt), data), (op_i, tt))
+  assoc >>>         ((key, tt), (data, (op_i, tt)))
+  first swap >>>    ((tt, key), (data, (op_i, tt)))
+  assoc >>>         (tt, (key, (data, (op_i, tt))))
+  second
+    (copy >>>
+     first f0) >>>  (tt, (f0 (key, (data, (op_i, tt)))),
+                             (key, (data, (op_i, tt))))
+  second
+    (copy >>>
+     first f) >>>   (tt, (f (f0 kdou, kdou), (f0 kdou, kdou))
+  unassoc >>>       ((tt, f (f0 kdou, kdou)), (f0 kdou, kdou))
+  first swap >>>    ((f (f0 kdou, kdou), tt), (f0 kdou, kdou))
+  second drop >>>   ((f (f0 kdou, kdou), tt), tt)
+  cancelr >>>       (f (f0 kdou, kdou), tt)
+  flatten
+     *)
+    
+    
+    rewrite cancelr_flatten.
+    .
